\subsection{Problem~1}%
\label{problem:1}

Solve the system and find the pivots when:
\begin{equation*}
    \systeme{2u-v=0,-u+2v-w=0,-v+2w-z=0,-w+2z=5}
\end{equation*}

\subsubsection*{Mathematics}
The solution to a linear system $\matr{A}x = \matr{b}$, where $\matr{A}$ is a
coefficient matrix and $\matr{b}$ is a column vector may be found by:
\begin{enumerate}
  \item Composing an augmented matrix
    $\matr{B} = \begin{amatrix}{1}{1}
      \matr{A} & \matr{b}
    \end{amatrix}$.
  \item Reducing the matrix $\matr{B}$ to the upper triangular form with the Gaussian
    Elimination\footnote{\nameref{algorithm:1}} algorithm.
  \item Obtaining the solution with the Back
    Substitution\footnote{\nameref{algorithm:4}} algorithm.
\end{enumerate}

Note, that this method works only when none of the $a_{ii}$ is zero, which is further
discussed in \nameref{problem:2}.

\subsubsection*{Solution}

Following the manual calculations of the Gaussian Elimination, we transform the matrix
to the upper triangular form:
\begin{equation*}
\begin{split}
    \begin{amatrix}{1}{1}
        \matr{A} & \matr{b}
    \end{amatrix} = 
    \begin{amatrix}{4}{1}
        \phantom{-}2 & -1 & \phantom{-}0 & \phantom{-}0 & 0\\
        -1 & \phantom{-}2 & -1 & \phantom{-}0 & 0\\
        \phantom{-}0 & -1 & \phantom{-}2 & -1 & 0\\
        \phantom{-}0 & \phantom{-}0 & -1 & \phantom{-}2 & 5
    \end{amatrix} &\xrightarrow{R_2 + \frac{1}{2}R_1} 
    \begin{amatrix}{4}{1}
        \phantom{-}2 & -1 & \phantom{-}0 & \phantom{-}0 & 0\\
        \phantom{-}0 & \phantom{-}\frac{3}{2} & -1 & \phantom{-}0 & 0\\
        \phantom{-}0 & -1 & \phantom{-}2 & -1 & 0\\
        \phantom{-}0 & \phantom{-}0 & -1 & \phantom{-}2 & 5
    \end{amatrix} \xrightarrow{R_3 + \frac{2}{3}R_2} \\
    \xrightarrow{R_3 + \frac{2}{3}R_2}
    \begin{amatrix}{4}{1}
        \phantom{-}2 & -1 & \phantom{-}0 & \phantom{-}0 & 0\\
        \phantom{-}0 & \phantom{-}\frac{3}{2} & -1 & \phantom{-}0 & 0\\
        \phantom{-}0 & \phantom{-}0 & \phantom{-}\frac{4}{3} & -1 & 0\\
        \phantom{-}0 & \phantom{-}0 & -1 & \phantom{-}2 & 5
    \end{amatrix} &\xrightarrow{R_4 + \frac{3}{4}R_3}
    \begin{amatrix}{4}{1}
        \phantom{-}2 & -1 & \phantom{-}0 & \phantom{-}0 & 0\\
        \phantom{-}0 & \phantom{-}\frac{3}{2} & -1 & \phantom{-}0 & 0\\
        \phantom{-}0 & \phantom{-}0 & \phantom{-}\frac{4}{3} & -1 & 0\\
        \phantom{-}0 & \phantom{-}0 & \phantom{-}0 & \phantom{-}\frac{5}{4} & 5
    \end{amatrix}
  \end{split}
\end{equation*}
and then we obtain the variables' values with the Back Substitution:
\begin{equation*}
  \begin{split}
    \systeme{2u-v=0,\frac{3}{2}v-2w=0,\frac{4}{3}w-z=0,\frac{5}{4}z=5}
    &\rightarrow
    \systeme{2u-v=0,\frac{3}{2}v-2w=0,\frac{4}{3}w-4=0,z=4}
    \rightarrow\\
    \rightarrow
    \systeme{2u-v=0,\frac{3}{2}v-6=0,w=3,z=4}
    &\rightarrow
    \systeme{2u-v=0,v=2,w=3,z=4}
    \rightarrow
    \systeme{u=1,v=2,w=3,z=4}
    \rightarrow
    \begin{cases}
    u=1\\
    v=2\\
    w=3\\
    z=4
    \end{cases}
\end{split}
\end{equation*}

Verifying the above calculation with our implementations in \MATLAB yields:
\lstinputlisting[style=Matlab-editor]{problems/Problem_1.m}
which corresponds to our solution.
